\documentclass{article}
\usepackage[utf8]{inputenc}
\usepackage{url}
\usepackage{hyperref}
\usepackage{amsmath}
\usepackage{mathpazo}
\usepackage{mathtools}
\usepackage{pst-text}
\usepackage{eepic}
\usepackage{pstricks}
\usepackage{tikz}

\begin{document}
\title{Trigonometric functions}
\author{}
\maketitle
\bibliographystyle{plain}

\section{Definitions}\cite{wiki:tri_func}

\setlength{\unitlength}{1cm}
\begin{picture}(0,4)
% Right-angled triangle
\put(1,0){\line(0,1){4}}
\put(1,0){\line(1,0){3}}
\put(1,4){\line(3,-4){3}}

\put(0.7,3.8){$A$}
\put(0.7,0.0){$C$}
\put(4.1,0.0){$B$}
\put(2.5,-0.2){$a$}
\put(0.7,2){$b$}
\put(2.8,2){$h \textit{ (hypotenuse)}$}

% Unit-circle
\put(7,2){\circle{4}}
\put(5,2){\line(1,0){4}}
\put(7,2){\line(1,1){2}}
\put(9,0){\line(0,1){4.5}}
\put(8.414,2){\line(0,1){1.414}}

\put(8.20,3.6){$\sec \theta$}
\put(8.20,2.5){$\sin \theta$}
\put(9.30,2.5){$\tan \theta$}

\end{picture}

This document using typesetting systems \LaTeX{} \cite{wiki:latex}.

\begin{align*}
  \tan \theta = \frac{\sin \theta}{\cos \theta},\,
  \cot \theta = \frac{1}{\tan \theta} = \frac{\cos \theta}{\sin \theta}\\
  \sec \theta = \frac{1}{\sin \theta},\,
  \csc \theta = \frac{1}{\cos \theta}
\end{align*}

\subsection{Series definitions}


\begin{align*}
  sin(x) &= x - {x^3 \over 3!} + {x^5 \over 5!} - {x^7 \over 7!} + ... =
           \sum_{n=0}^\infty {(-1)^n \over (2n+1)!} x^{2n+1}\\
  cos(x) &= 1 - {x^2 \over 2!} + {x^4 \over 4!} - {x^6 \over 6!} + ... =
           \sum_{n=0}^\infty {(-1)^n \over (2n)!} x^{2n}\\
\end{align*}

\section{Identites}

\subparagraph{Pythagorean identity}
\begin{align*}
  \sin^2 \theta +   \cos^2 \theta = 1\\
  \implies 1 + \tan^2 \theta = \sec^2 \theta\\
  \implies 1 + \cot^2 \theta = \csc^2 \theta
\end{align*}

\subparagraph{Symmetry, shifts, and periodicity}
\textbf{Symmetry}


\subparagraph{Angle sum and difference identities}

\begin{align*}
  \sin(\alpha \pm \beta) = \sin\alpha \cos\beta \pm \cos\alpha \sin\beta\\
  \cos(\alpha \pm \beta) = \cos\alpha \cos\beta \mp \sin\alpha \sin\beta
\end{align*}

\subparagraph{Product-to-sum and sum-to-product identities}
\begin{align*}
   2 \cos \alpha \cos \beta = \cos(\alpha - \beta) + \cos(\alpha + \beta)\\
   2 \sin \alpha \sin \beta = \cos(\alpha - \beta) - \cos(\alpha + \beta)\\
   2 \sin \alpha \cos \beta = \sin(\alpha + \beta) + \sin(\alpha + \beta)\\
   2 \cos \alpha \sin \beta = \sin(\alpha + \beta) - \sin(\alpha + \beta)
\end{align*}

\bibliography{math}
\end{document}

%%% Local Variables:
%%% mode: latex
%%% TeX-master: t
%%% End:
